wip

src/matroid/minor'.lean
@@ -1,3 +1,5 @@
+/-  An alternative take on the definition of a minor, where we take a quotient. Very much WIP. -/
+
 import ftype.basic ftype.embed set_tactic.solver
 import .rankfun .dual 
 
@@ -9,13 +11,11 @@ open ftype
 
 variables {U₀ U V W: ftype}--[nonempty U₀]
 
-namespace function.embedding
+--def img (emb : U₀ ↪ U):=
+--  λ (X : set U₀), emb.to_fun '' X 
 
-def img (emb : U₀ ↪ U):=
-  λ (X : set U₀), emb.to_fun '' X 
-
-/-- given an injection emb, and a set equal to the range of emb, outputs an equivalence between the 
-domain and the subtype corresponding to the range. -/ 
+/- given an injection emb, and a set equal to the range of emb, outputs an equivalence between the 
+domain and the subtype corresponding to the range. 
 def subtype_inv_inj (emb : U₀ ↪ U){E : set U}(hE : E = set.range emb) : E ≃ U₀ :=   
 let h : Π (y : E), (∃ x : U₀, emb x = y) := 
   by {rintros ⟨y,hy⟩, rw [hE, set.mem_range] at hy, cases hy with x hx, from ⟨x, by simp [hx]⟩},
@@ -27,24 +27,14 @@ let h : Π (y : E), (∃ x : U₀, emb x = y) :=
   left_inv := by {intros y, simp_rw (desc y).property, simp}, 
   right_inv := λ x, by {cases emb with f h_inj, from h_inj (desc ⟨f x,_⟩).property},
 }
+-/
 
-end function.embedding 
 
-
-namespace equiv 
-
-def img (bij : U ≃ V) :=
-  λ (X : set U), bij.to_fun '' X 
-
-def inv_img (bij : U ≃ V) :=
-  λ (X : set V), bij.to_fun ⁻¹' X
-
-end equiv 
 
 /-- bundled isomorphism between two matroids -/
 structure isom (M : matroid U)(N : matroid V) := 
   (bij: U ≃ V)
-  (rank_preserving : M.r =  N.r ∘ bij.img)
+  (rank_preserving : M.r =  N.r ∘ (set.image bij))
 
 instance coe_iso_to_fun {M : matroid U}{N : matroid V}: has_coe_to_fun (isom M N) := 
 {F := λ (i : isom M N), (U → V), coe := λ i, i.bij}
@@ -54,7 +44,7 @@ def inv{M: matroid U}{N: matroid V}(iso : isom M N) : isom N M :=
 {
   bij := iso.bij.symm,
   rank_preserving := 
-  by {rw iso.rank_preserving, unfold equiv.img, ext X, convert rfl, convert rfl, ext x, simp}, 
+  by {rw iso.rank_preserving, ext X, convert rfl, convert rfl, ext x, simp}, 
 }
 
 def compose {M : matroid U}{N : matroid V}{O : matroid W}(i₁ : isom M N)(i₂ : isom N O): isom M O := 
@@ -63,16 +53,16 @@ def compose {M : matroid U}{N : matroid V}{O : matroid W}(i₁ : isom M N)(i₂ 
   rank_preserving := 
   begin
     ext X, rw [i₁.rank_preserving, i₂.rank_preserving],  
-    simp only [equiv.to_fun_as_coe, ftype.ftype_coe, function.comp_app, equiv.coe_trans, equiv.img], 
+    simp only [equiv.to_fun_as_coe, ftype.ftype_coe, function.comp_app, equiv.coe_trans], 
     apply congr_arg, ext x,  simp, 
   end
 }
 
 -- making a hash of this one! 
 @[simp] lemma compose_inv_on_set {M: matroid U}{N: matroid V}(iso : isom M N)(X : set U):
-  ((inv iso).bij.img (iso.bij.img X)) = X :=
+  ((inv iso).bij '' (iso.bij '' X)) = X :=
 begin
-  unfold equiv.img, 
+  --unfold equiv.img, 
   convert rfl, ext, 
   rw set.mem_image, 
   refine ⟨λ h, ⟨iso.bij x,⟨_,_⟩⟩,λ h, _⟩, 
@@ -87,23 +77,167 @@ variable {M : matroid U}
 
 
 
-/-- structure describing a matroid together with it having an isomorphism to a minor of M -/
-structure emb_mat := 
+/-- structure describing a matroid and an embedding of its elements into U -/
+structure emb_mat (U : ftype) := 
   {U₀ : ftype}
   (mat : matroid U₀)
   (emb : U₀ ↪ U)
 
-structure emb_minor (M : matroid U):=
+namespace emb_mat 
+
+def ground (N : emb_mat U) : set U := 
+  set.range N.emb 
+
+def strongly_iso (N₁ N₂ : emb_mat U) : Prop := 
+  (∃ (φ : isom (N₁.mat) (N₂.mat)), ∀ x, N₁.emb x = N₂.emb (φ x)) 
+
+lemma strong_iso_equiv : 
+  equivalence (λ (N₁ N₂ : emb_mat U), strongly_iso N₁ N₂) := 
+begin
+  refine ⟨λ N, _, λ N₁ N₂ hab, _, λ N₁ N₂ N₃ hab hbc, _⟩, 
+    {refine ⟨⟨equiv.refl _,_⟩,λ X, _⟩, 
+      {ext X, simp,},
+      {apply congr_arg, unfold_coes, simp} },
+    {cases hab with φ, refine ⟨inv φ, λ X, _⟩, rw [hab_h ((inv φ) X), inv], unfold_coes, simp},
+  cases hab with i₁ h₁, cases hbc with i₂ h₂, 
+  from ⟨compose i₁ i₂, λ X, by {unfold_coes at *, simp [h₁,h₂,congr_arg, compose]}⟩,  
+end
+
+lemma strong_iso_same_groundset (N N' : emb_mat U):
+  strongly_iso N N' → N.ground = N'.ground  := 
+begin
+  rintros ⟨h₁,h₂⟩, ext, 
+  simp only [ground, set.mem_range],
+  simp_rw h₂, 
+  refine ⟨λ h, _, λ h, _⟩, 
+    {cases h with y hy, from ⟨_, hy⟩},
+  cases h with y hy, use h₁.bij.inv_fun y, unfold_coes, simp [hy],
+end 
+
+--def pullback_r (N : emb_mat U) : set (N.ground) → ℤ := 
+--  λ X, N.mat.r ((N.emb.subtype_inv_inj (rfl : N.ground = set.range N.emb))'' X)
+
+/-- mapped rank function of N, but defined on all subsets of U (elements not in image are ignored)-/
+def pullback_r (N : emb_mat U) : set U → ℤ := 
+  λ X, N.mat.r ({x : N.U₀ | N.emb x ∈ X })
+
+lemma pullback_r_eq (N : emb_mat U)(X : set N.U₀) : 
+  N.mat.r X = N.pullback_r (N.emb.to_fun '' X) :=
+begin
+  unfold pullback_r, congr', ext x, 
+  simp only [set.mem_image, function.embedding.to_fun_eq_coe, set.mem_set_of_eq],
+  refine ⟨λ h, _, λ h, _⟩, 
+    {use x, simp, from h},
+  cases h with x' hx', 
+  convert hx'.1,
+  from (N.emb.inj' hx'.2).symm,
+end
+  --ite (X ⊆ N.ground) (some 0 : option ℤ) (none : option ℤ) 
+  
+  --N.mat.r ((N.emb.subtype_inv_inj (rfl : N.ground = set.range N.emb))'' X)
+
+lemma strong_iso_same_pullback_r (N N' : emb_mat U):
+  strongly_iso N N' → N.pullback_r = N'.pullback_r :=
+begin
+  rintros ⟨⟨φ,hφ₁⟩, hφ₂⟩, ext X, 
+  unfold pullback_r, rw hφ₁, 
+  dsimp, congr', ext x', 
+  simp only [set.mem_image, set.mem_set_of_eq], 
+  simp_rw hφ₂, 
+  refine ⟨λ h, _, λ h, ⟨φ.inv_fun x',⟨_,by simp⟩⟩⟩, 
+    {rcases h with ⟨x, ⟨hx₁,hx₂⟩⟩, rw ←hx₂, from hx₁,},
+  rw ←hφ₂, 
+  convert h,  
+  rw hφ₂, 
+  congr', unfold_coes, simp, 
+end
+
+/-- if E is equal to the groundset of N, then there is a natural equivalence between E and U₀ -/
+def groundset_equiv (N : emb_mat U){E : set U}(hE : N.ground = E): 
+  E ≃ N.U₀ := 
+  ((equiv.set.range N.emb N.emb.inj').trans (equiv.set.of_eq hE)).symm 
+
+--def pullback_r' (N : emb_mat U){E : set U}(hE : N.ground = E) : set E → ℤ := 
+
+
+
+instance strong_iso_setoid (U : ftype) : setoid (emb_mat U) := ⟨strongly_iso, strong_iso_equiv⟩ 
+
+end emb_mat 
+
+/-- a matroid_in U is a matroid embedded into some set of elements of U, modulo the range of the embedding-/
+def matroid_in (U : ftype) := quot (λ (N N' : emb_mat U), N.strongly_iso N')
+
+namespace matroid_in 
+
+def ground : matroid_in U → set U := quotient.lift  
+  (λ (N : emb_mat U), N.ground) emb_mat.strong_iso_same_groundset
+
+def ground_ftype (N : matroid_in U) : ftype := ⟨N.ground⟩
+
+def r : matroid_in U → (set U → ℤ) := quotient.lift 
+  (λ (N : emb_mat U), N.pullback_r) emb_mat.strong_iso_same_pullback_r
+
+def r_subtype (N : matroid_in U) : (set (N.ground) → ℤ) := 
+  λ X, N.r (coe '' X)
+
+--def rep_spec (N : matroid_in U) : {N₀ : emb_mat U // ⟦N₀⟧ = N} := 
+--  classical.indefinite_description _ (quot.exists_rep N)
+
+/- The rank axioms should be provable here, but stuck in quotient hell. -/
+def as_matroid (N : matroid_in U) : matroid (N.ground_ftype) := 
+--let N₀ := rep_spec N in 
+{ 
+  r := N.r_subtype,
+  R0 := 
+  begin
+  cases quot.exists_rep N with N₀ hN₀,  
+  intro X, 
+  simp only [matroid_in.r_subtype, matroid_in.r], 
+  have := quotient.lift_beta (λ (N : emb_mat U), N.pullback_r) emb_mat.strong_iso_same_pullback_r N₀ , 
+  dsimp only [quotient.mk] at this hN₀, simp_rw [←hN₀, this],
+  
+    --simp [matroid_in.r_subtype], intro X, dsimp, 
+    --have := N₀.2, 
+    --have n := N₀.1, 
+    --have := n.mat.R0, 
+  end ,
+  R1 := sorry ,
+  R2 := sorry ,
+  R3 := sorry 
+}
+
+
+
+def is_minor (N : matroid_in U)(M : matroid U) := 
+  ∃ C, C ∩ N.ground = ∅ ∧ (∀ X ⊆ N.ground, N.r X = M.r (X ∪ C) - M.r C) 
+
+def is_minor_nested (N M : matroid_in U) : Prop := 
+  (N.ground ⊆ M.ground) ∧ ∃ C ⊆ M.ground \ N.ground, (∀ X ⊆ N.ground, N.r X = M.r (X ∪ C) - M.r C)  
+
+
+/- the rank function given by N when applied to a subset of the embedded ground set of N.  -/
+
+
+--def is_minor (N : emb_mat U)(M : matroid U) := 
+  --∃ C, C ∩ N.ground = ∅ ∧ ∀ X : set U₀, N.mat.r 
+
+end matroid_in
+
+--def is_minor {U : ftype}(N : emb_mat U)(M : matroid U) := 
+--  ∃ C : set U, C ∩ N.ground = ∅ ∧ ∀ 
+
+/-structure emb_minor' (M : matroid U):=
   {U₀ : ftype}
   (mat : matroid U₀)
   (emb : U₀ ↪ U)
   (C : set U)
   (C_disj : C ∩ set.range emb = ∅)
-  (minor_rank : mat.r = λ X, M.r (emb '' X ∪ C) - M.r C)
+  (minor_rank : mat.r = λ X, M.r (emb '' X ∪ C) - M.r C)-/
 
-namespace emb_minor
 
-/-- the ground set of an emb_minor, expressed as a set of elements of M -/
+/-
+/- the ground set of an emb_minor, expressed as a set of elements of M -/
 def ground (N : emb_minor M) : set U := set.range N.emb
 
 --def C (N : emb_minor M) : set U := classical.some N.minor_rank
@@ -118,8 +252,7 @@ by {rw ground, from N.C_disj,}
 
 lemma D_ground_inter_empty (N : emb_minor M): 
   N.D ∩ N.ground = ∅ := 
-by {rw [D], have := C_ground_inter_empty N, set_solver}
-  -- set_solver doesn't work right after the have here, but it should. What's the problem? 
+by {rw [D], have := C_ground_inter_empty N, set_solver,}
 
 lemma C_D_inter_empty (N : emb_minor M) : 
   N.C ∩ N.D = ∅ := 
@@ -128,22 +261,21 @@ by {rw D, have := C_ground_inter_empty N, set_solver,}
 lemma C_union_D_eq_ground_compl (N : emb_minor M) : 
   (N.C ∪ N.D) = N.groundᶜ := 
 by {rw [D], have := N.C_ground_inter_empty, set_solver,}
--- same deal here 
 
 lemma emb_minor_r (N : emb_minor M)(X : set N.U₀): 
   N.mat.r X = M.r (N.emb '' X ∪ N.C) - M.r N.C := 
 by rw N.minor_rank
 
-/-- the rank function given by N when applied to a subset of the embedded ground set of N.  -/
+/- the rank function given by N when applied to a subset of the embedded ground set of N.  -/
 def pullback_r (N : emb_minor M) : set (N.ground) → ℤ := 
   λ X, N.mat.r ((N.emb.subtype_inv_inj (rfl : N.ground = set.range N.emb))'' X)
 
-/-- two embedded minors of M are strongly isomorphic if the associated matroids are related 
+/- two embedded minors of M are strongly isomorphic if the associated matroids are related 
 by an isomorphism that commutes with the respective embeddings into M. -/
 def strongly_iso (N₁ N₂ : emb_minor M) : Prop := 
   (∃ (φ : isom (N₁.mat) (N₂.mat)), ∀ x, N₁.emb x = N₂.emb (φ x)) 
 
-/-- existence of a strong isomorphism is an equivalence relation on embedded minors of M.
+/- existence of a strong isomorphism is an equivalence relation on embedded minors of M.
     Equivalence classes of this relation correspond to actual 'labelled' minors of M    -/
 lemma strong_iso_equiv : 
   equivalence (λ (N₁ N₂ : emb_minor M), strongly_iso N₁ N₂) := 
@@ -157,7 +289,7 @@ begin
   from ⟨compose i₁ i₂, λ X, by {unfold_coes at *, simp [h₁,h₂,congr_arg, compose]}⟩,  
 end
 
-/-- the ground set is an invariant of equivalence classes under strong isomorphism -/
+/- the ground set is an invariant of equivalence classes under strong isomorphism -/
 lemma strong_iso_same_groundset (N N' : emb_minor M):
   strongly_iso N N' → N.ground = N'.ground  := 
 begin
@@ -183,9 +315,11 @@ namespace minor
 
 def emb_to_minor (M : matroid U) := @quotient.mk (emb_minor M) _
 
-/-- returns the ground set of a minor of M (as a subset of the ftype for M) -/
+/- returns the ground set of a minor of M (as a subset of the ftype for M) -/
 def ground {M : matroid U} : minor M → set U := quotient.lift  
   (λ (N : emb_minor M), N.ground )
   (λ N N' hNN', emb_minor.strong_iso_same_groundset N N' hNN' )
 
 end minor 
+
+-/
